fix br93

examples/br93.ec
@@ -92,30 +92,7 @@ hint simplify cost_f.
 (* (we simply instantiate the generic theory of Random Oracles with     *)
 (*    the types and output distribution declared above, discharging all *)
 (*          assumptions on the instantiated parameters--there are none) *)
-<<<<<<< HEAD
-clone import ROM.Lazy as H with
-  type from  <- rand,
-  type to    <- ptxt,
-  op dsample <- fun _ => dptxt
-proof *.
 
-clone import FMapCost as FMC with
-  type from  <- rand.
-
-module type HASH = {
-  proc init(): unit
-  proc hash(x:rand): ptxt
-}.
-
-(* Specializing and merging the hash function *)
-
-module Hash = {
-  var qs : rand list
-  proc init(): unit = { RO.init(); qs <- []; }
-  proc o(x:rand): ptxt = { var y; qs <- x::qs; y <@ RO.o(x); return y; }
-  proc hash = RO.o
-}.
-=======
 clone import ROM as H with
   type in_t    <- rand,
   type out_t   <- ptxt,
@@ -123,13 +100,16 @@ clone import ROM as H with
   type d_out_t <- bool,
   op   dout _  <- dptxt.
 import H.Lazy.
->>>>>>> origin/1.0-preview
+
+clone import FMapCost as FMC with
+  type from  <- rand.
 
 (* We can define the Bellare-Rogaway 93 PKE Scheme.                     *)
 (* BR93 is a module that, given access to an oracle H from type         *)
 (*   `from` to type `rand` (see `print Oracle.`), implements procedures *)
 (*   `keygen`, `enc` and `dec` as follows described below.              *)
-module BR93 (H:HASH) = {
+
+module BR93 (H:Oracle) = {
   (* `keygen` simply samples a key pair in `dkeys` *)
   proc kg() = {
     var kp;
@@ -147,7 +127,7 @@ module BR93 (H:HASH) = {
     var r, h;
 
     r <$ drand;
-    h <@ H.hash(r);
+    h <@ H.o(r);
     return (f pk r,h +^ m);
   }
 
@@ -161,7 +141,7 @@ module BR93 (H:HASH) = {
 
     (r,m) <- c;
     r     <- fi sk r;
-    h     <- H.hash(r);
+    h     <- H.o(r);
     return h +^ m;
   }
 }.
@@ -178,15 +158,9 @@ module Correctness = {
   proc main(m) = {
     var pk, sk, c, m';
 
-<<<<<<< HEAD
-    (pk,sk) <@ BR93(Hash).kg();
-    c       <@ BR93(Hash).enc(pk,m);
-    m'      <@ BR93(Hash).dec(sk,c);
-=======
-    (pk,sk) <@ BR93(LRO).keygen();
+    (pk,sk) <@ BR93(LRO).kg();
     c       <@ BR93(LRO).enc(pk,m);
     m'      <@ BR93(LRO).dec(sk,c);
->>>>>>> origin/1.0-preview
     return (m = m');
   }
 }.
@@ -195,19 +169,14 @@ lemma BR93_correct &m m: Pr[Correctness.main(m) @ &m: res] = 1%r.
 proof.
 byphoare=> //; conseq (: _ ==> true) (: _ ==> res)=> //.
 + proc; inline *.
-  rcondf 19.
+  rcondf 18.
   + auto=> /> [pk sk] kp_in_dkeys r _ y _ /=.
     rewrite fK //; split=> [_ _ _|-> //].
     by rewrite mem_set.
   auto=> /> &hr [pk sk] kp_in_dkeys r _ y _ /=.
   rewrite fK //; split=> [_ y' _|].
   + by rewrite get_set_sameE -addA addKp.
-<<<<<<< HEAD
   + by rewrite mem_empty.
-=======
-  rewrite domE; case: (LRO.m{hr}.[r])=> [|p] //= _ _.
-  by rewrite -addA addKp.
->>>>>>> origin/1.0-preview
 by proc; inline *; auto=> />; rewrite dkeys_ll drand_ll dptxt_ll.
 qed.
 
@@ -230,16 +199,11 @@ realize challenge_ll by move=> _ _; exact/drand_ll.
 realize challenge_uni by move=> _ _; exact/drand_uni.
 realize finvof by move=> pk sk x /fK ->.
 
-<<<<<<< HEAD
-module type Adv (ARO: ARO)  = {
-  proc choose(p:pkey): (ptxt * ptxt)
-  proc guess(c:ctxt): bool
-=======
 (* But we can't do it (yet) for IND-CPA because of the random oracle    *)
 (*             Instead, we define CPA for BR93 with that particular RO. *)
 module type Adv (ARO: POracle)  = {
-  proc a1(p:pkey): (ptxt * ptxt)
-  proc a2(c:ctxt): bool
+  proc choose(p:pkey): (ptxt * ptxt)
+  proc guess(c:ctxt): bool
 }.
 
 (* We need to log the random oracle queries made to the adversary       *)
@@ -266,38 +230,29 @@ module BR93_CPA(A:Adv) = {
     var pk, sk, m0, m1, c, b, b';
 
                 Log(LRO).init();
-    (pk,sk)  <@ BR93(LRO).keygen();
-    (m0,m1)  <@ A(Log(LRO)).a1(pk);
+    (pk,sk)  <@ BR93(LRO).kg();
+    (m0,m1)  <@ A(Log(LRO)).choose(pk);
     b        <$ {0,1};
     c        <@ BR93(LRO).enc(pk,b?m0:m1);
-    b'       <@ A(Log(LRO)).a2(c);
+    b'       <@ A(Log(LRO)).guess(c);
     return b' = b;
   }
->>>>>>> origin/1.0-preview
 }.
 
 (* We want to prove the following:                                      *)
 (*   forall (valid) CPA adversary A which makes at most q queries to H, *)
 (*     there exists a OW adversary I such that                          *)
 (*          `|Pr[CPA(BR, A): res] - 1/2| <= Pr[OW_f(I): res]             *)
-(* We construct I as follows, using A.a1 and A.a2 as black boxes        *)
+(* We construct I as follows, using A.choose and A.guess as black boxes        *)
 module I(A:Adv): Inverter = {
   proc invert(pk:pkey,y:rand): rand = {
     var m0, m1, h, b, x;
 
-<<<<<<< HEAD
-               Hash.init();
-    (m0,m1) <@ A(Hash).choose(pk);
-    h       <$ dptxt;
-    b       <@ A(Hash).guess(y,h);
-    x       <- nth witness Hash.qs (find (fun p => f pk p = y) Hash.qs);
-=======
                Log(LRO).init();
-    (m0,m1) <@ A(Log(LRO)).a1(pk);
+    (m0,m1) <@ A(Log(LRO)).choose(pk);
     h       <$ dptxt;
-    b       <@ A(Log(LRO)).a2(y,h);
+    b       <@ A(Log(LRO)).guess(y,h);
     x       <- nth witness Log.qs (find (fun p => f pk p = y) Log.qs);
->>>>>>> origin/1.0-preview
 
     return x;
   }
@@ -306,16 +261,10 @@ module I(A:Adv): Inverter = {
 (* We now prove the result using a sequence of games                    *)
 section.
 (* All lemmas in this section hold for all (valid) CPA adversary A      *)
-<<<<<<< HEAD
-declare module A : Adv { -Hash }.
 
-axiom A_guess_ll (O <: ARO {-A}): islossless O.o => islossless A(O).guess.
-=======
-declare module A : Adv { LRO, Log }.
+declare module A : Adv { -LRO, -Log }.
 
-axiom A_a1_ll (O <: POracle {A}): islossless O.o => islossless A(O).a1.
-axiom A_a2_ll (O <: POracle {A}): islossless O.o => islossless A(O).a2.
->>>>>>> origin/1.0-preview
+axiom A_guess_ll (O <: POracle {-A}): islossless O.o => islossless A(O).guess.
 
 (* Step 1: replace RO call with random sampling                         *)
 local module Game1 = {
@@ -323,101 +272,39 @@ local module Game1 = {
 
   proc main() = {
     var pk, sk, m0, m1, b, h, c, b';
-<<<<<<< HEAD
-                Hash.init();
-    (pk,sk)  <$ dkeys;
-    (m0,m1)  <@ A(Hash).choose(pk);
-=======
                 Log(LRO).init();
     (pk,sk)  <$ dkeys;
-    (m0,m1)  <@ A(Log(LRO)).a1(pk);
->>>>>>> origin/1.0-preview
+    (m0,m1)  <@ A(Log(LRO)).choose(pk);
     b        <$ {0,1};
-
     r        <$ drand;
     h        <$ dptxt;
     c        <- ((f pk r),h +^ (b?m1:m0));
-
-<<<<<<< HEAD
-    b'       <@ A(Hash).guess(c);
-=======
-    b'       <@ A(Log(LRO)).a2(c);
->>>>>>> origin/1.0-preview
+    b'       <@ A(Log(LRO)).guess(c);
     return b' = b;
   }
 }.
 
+
 local lemma pr_Game0_Game1 &m:
-     Pr[CPA(BR93(Hash), A(Hash)).main() @ &m: res]
+     Pr[CPA(BR93(LRO), A(LRO)).main() @ &m: res]
   <=   Pr[Game1.main() @ &m: res]
-     + Pr[Game1.main() @ &m: Game1.r \in Hash.qs].
+     + Pr[Game1.main() @ &m: Game1.r \in Log.qs].
 proof.
 byequiv=> //; proc.
-<<<<<<< HEAD
-inline BR93(Hash).enc BR93(Hash).kg.
+inline BR93(LRO).enc BR93(LRO).kg.
 (* Until the replaced RO call, the two games are in sync.               *)
 (*        In addition, the log's contents coincide with the RO queries. *)
-call (_: Game1.r \in Hash.qs,
-         (forall x, x \in Hash.qs{2} = x \in RO.m{2}) /\
-         eq_except (pred1 Game1.r{2}) RO.m{1} RO.m{2}).
+call (_: Game1.r \in Log.qs,
+         (forall x, x \in Log.qs{2} = x \in LRO.m{2}) /\
+         eq_except (pred1 Game1.r{2}) LRO.m{1} LRO.m{2}).
 + by apply A_guess_ll.
 + by proc; inline *; auto => /> &1 &2 hb; smt (eq_except_set_eq get_setE).
 + by move=> *; islossless.
 + by move=> /=; proc; call (_: true); 1: islossless; auto => />.
-inline Hash.hash; auto => /=.
-call (_: ={glob Hash} /\ (forall x, x \in Hash.qs{2} = x \in RO.m{2})).
+inline LRO.o; auto => /=.
+call (_: ={glob LRO} /\ (forall x, x \in Log.qs{2} = x \in LRO.m{2})).
 + by proc; inline *;auto => />; smt (get_setE).
 by inline *;auto => />; smt (mem_empty eq_except_setl get_setE).
-=======
-inline BR93(LRO).enc BR93(LRO).keygen.
-(* Until the replaced RO call, the two games are in sync.               *)
-(*        In addition, the log's contents coincide with the RO queries. *)
-seq  8  5: (   ={glob A, glob LRO, glob Log, pk, sk, b}
-            /\ pk0{1} = pk{2}
-            /\ m{1} = (b?m0:m1){2}
-            /\ r{1} = Game1.r{2}
-            /\ (forall x, x \in Log.qs{1} <=> x \in LRO.m{1})).
-+ auto; call (:   ={glob Log, glob LRO}
-               /\ (forall x, x \in Log.qs{1} <=> x \in LRO.m{1})).
-  + proc; inline LRO.o.
-    by auto=> /> &2 log_is_dom y _; smt(@SmtMap).
-  by inline *; auto=> /> _ _ x; rewrite mem_empty.
-(* We now deal with everything that happens after the programs differ: *)
-(*   - until r gets queried to the random oracle by the adversary      *)
-(*     (and if it wasn't already queried by a1), we guarantee that the *)
-(*     random oracles agree except on r                                *)
-(*   - if the adversary queries r to the random oracle (or if it has   *)
-(*     already done so in a1), we give up                              *)
-(* Because we reason up to bad, we need to prove that bad is stable    *)
-(* and that the adversary and its oracles are lossless                 *)
-call (_: Game1.r \in Log.qs,
-         eq_except (pred1 Game1.r{2}) LRO.m{1} LRO.m{2}).
-+ exact/A_a2_ll.
-+ proc; inline LRO.o.
-  auto=> /> &1 &2 _ m1_eqe_m2 yL y_in_dptxt; split.
-  + move=> x_notin_m; split.
-    + by rewrite !get_set_sameE eq_except_set_eq.
-    move: m1_eqe_m2 x_notin_m=> + + + r_neq_x.
-    by rewrite eq_exceptP pred1E !domE=> /(_ x{2} r_neq_x) ->.
-  move=> x_in_m; split.
-  + move: m1_eqe_m2 x_in_m=> + + + r_neq_x.
-    by rewrite eq_exceptP pred1E !domE=> /(_ x{2} r_neq_x) ->.
-  by move: m1_eqe_m2=> + _ r_neq_x- /eq_exceptP /(_ x{2}); rewrite pred1E=> /(_ r_neq_x) ->.
-+ by move=> &2 _; proc; call (LRO_o_ll _); auto=> /=; apply: dptxt_ll.
-+ move=> _ /=; proc; inline *.
-  conseq (: true ==> true: =1%r) (: Game1.r \in Log.qs ==> Game1.r \in Log.qs)=> //=.
-  + by auto=> />.
-  by auto=> />; exact/dptxt_ll.
-inline LRO.o; case: ((r \in LRO.m){1}).
-+ conseq (: _ ==> ={b} /\ Game1.r{2} \in Log.qs{2})=> //=.
-  + by move=> /> &1 &2 _ _ rR _ _ _ _ _ h /h [] -> //.
-  by auto=> /> &2 <- ->.
-rcondt{1} 3; 1:by auto.
-auto=> /> &2 log_is_dom r_notin_m y _; rewrite !get_set_sameE oget_some /=.
-split.
-+ by move=> _; rewrite eq_exceptP /pred1=> x; rewrite get_setE eq_sym=> ->.
-by move=> _ rR aL mL aR qsR mR h /h [] ->.
->>>>>>> origin/1.0-preview
 qed.
 
 (* Step 2: replace h ^ m with h in the challenge encryption            *)
@@ -426,45 +313,27 @@ local module Game2 = {
 
   proc main() = {
     var pk, sk, m0, m1, b, h, c, b';
-<<<<<<< HEAD
-                Hash.init();
-    (pk,sk)  <$ dkeys;
-    (m0,m1)  <@ A(Hash).choose(pk);
-    r        <$ drand;
-    h        <$ dptxt;
-    c        <- ((f pk r),h);
-    b'       <@ A(Hash).guess(c);
-    b        <$ {0,1};
-=======
                 Log(LRO).init();
     (pk,sk)  <$ dkeys;
-    (m0,m1)  <@ A(Log(LRO)).a1(pk);
+    (m0,m1)  <@ A(Log(LRO)).choose(pk);
     b        <$ {0,1};
 
     r        <$ drand;
     h        <$ dptxt;
     c        <- ((f pk r),h);
 
-    b'       <@ A(Log(LRO)).a2(c);
->>>>>>> origin/1.0-preview
+    b'       <@ A(Log(LRO)).guess(c);
     return b' = b;
   }
 }.
 
 local equiv eq_Game1_Game2: Game1.main ~ Game2.main:
-  ={glob A} ==> ={glob Hash, res} /\ Game1.r{1} = Game2.r{2}.
+  ={glob A} ==> ={glob Log, glob LRO, res} /\ Game1.r{1} = Game2.r{2}.
 proof.
-<<<<<<< HEAD
-proc. swap{2} -4.
-call (: ={glob Hash}); 1: by sim.
-wp; rnd (fun x=> x +^ (b?m1:m0){2}).
-auto; call (: ={glob Hash}); 1: by sim.
-=======
 proc.
 call (: ={glob Log, glob LRO}); 1: by sim.
-wp; rnd (fun x=> x +^ (b?m0:m1){2}).
+wp; rnd (fun x=> x +^ (b?m1:m0){2}).
 auto; call (: ={glob Log, glob LRO}); 1: by sim.
->>>>>>> origin/1.0-preview
 inline *; auto=> /> _ _ rR b _ rL _; split=> [|_].
 + by move=> hR _; rewrite addpK.
 by move=> hL _; rewrite addpK.
@@ -475,156 +344,47 @@ local lemma pr_Game1_Game2 &m:
 proof. by byequiv eq_Game1_Game2. qed.
 
 local lemma pr_bad_Game1_Game2 &m:
-    Pr[Game1.main() @ &m: Game1.r \in Hash.qs]
-  = Pr[Game2.main() @ &m: Game2.r \in Hash.qs].
+    Pr[Game1.main() @ &m: Game1.r \in Log.qs]
+  = Pr[Game2.main() @ &m: Game2.r \in Log.qs].
 proof. by byequiv eq_Game1_Game2. qed.
 
 local lemma pr_Game2 &m: Pr[Game2.main() @ &m: res] <= 1%r / 2%r.
 proof.
 byphoare=> //=; proc.
-<<<<<<< HEAD
-by rnd (pred1 b'); conseq (: true) => // /> *; rewrite dbool1E.
-=======
 swap 4 4.
 wp; rnd (pred1 b')=> //=.
-inline *; call (_: true).
-+ exact A_a2_ll. (* adversary *)
-+ by proc; call (LRO_o_ll _); auto=> /=; apply: dptxt_ll. (* oracle *)
-auto; call (_: true).
-+ exact A_a1_ll. (* adversary *)
-+ by proc; call (LRO_o_ll _); auto=> /=; apply: dptxt_ll. (* oracle *)
-auto=> />; rewrite dkeys_ll drand_ll dptxt_ll /predT /=.
-by move=> _ _ _ _ _ _ r; rewrite dbool1E pred1E.
->>>>>>> origin/1.0-preview
+conseq (:true) => //.
+by move=> *; rewrite dbool1E pred1E.
 qed.
 
 (* Step 3: The reduction step -- if A queries the RO with the randomness *)
 (*     used to encrypt the challenge, then I(A) inverts the OW challenge *)
 
 local lemma pr_Game2_OW &m:
-  Pr[Game2.main() @ &m: Game2.r \in Hash.qs]
+  Pr[Game2.main() @ &m: Game2.r \in Log.qs]
   <= Pr[OW(I(A)).main() @ &m: res].
 proof.
-<<<<<<< HEAD
 byequiv => //=; proc; inline *.
-swap{1} 5 -1.
-rnd{1}; wp.
-call (_: ={glob Hash}); 1: by sim.
+wp.
+call (_: ={glob Log, glob LRO}); 1: by sim.
+swap{1} 6 -2.
 auto.
-call (_: ={glob Hash}); 1: by sim.
-auto => /> -[pk sk] hkeys r _ h _ qs _ _ hin.
+call (_: ={glob Log, glob LRO}); 1: by sim.
+auto => /> -[pk sk] hkeys r _ _ _ h _ qs hin.
 pose P := fun p => f _ p = _.
 apply/(fI pk); 1: by exists sk.
 have <- // := (nth_find witness P qs _).
 by rewrite hasP; exists r.
-=======
-rewrite (OW_OWr &m (I(A))). (* Note: we proved it forall (abstract) I    *)
-byequiv => //=; proc; inline *; wp.
-conseq
-  (_ : _ ==>
-       support dkeys (pk0{2}, sk{2}) /\
-       Game2.r{1} = OWr.x{2} /\ Log.qs{1} = Log.qs{2} /\
-       y{2} = f pk0{2} Game2.r{1}).
-+ move=> /> qs x pk sk vk x_in_qs; pose P := fun p => f _ p = _.
-  have h := nth_find witness P qs _.
-  + by rewrite hasP; exists x.
-  apply/(fI pk).
-  + by exists sk.
-  by rewrite h.
-(* rest of proof *)
-call (: ={glob Log, glob LRO}); 1: by sim.
-swap{1} 6 -2.
-auto; call (: ={glob Log, glob LRO}); 1: by sim.
-by auto=> /> [pk sk] ->.
->>>>>>> origin/1.0-preview
 qed.
 
 lemma Reduction &m:
-  Pr[CPA(BR93(Hash), A(Hash)).main() @ &m : res] - 1%r/2%r
+  Pr[CPA(BR93(LRO), A(LRO)).main() @ &m : res] - 1%r/2%r
   <= Pr[OW(I(A)).main() @ &m: res].
 proof.
 smt(pr_Game0_Game1 pr_Game1_Game2 pr_bad_Game1_Game2 pr_Game2 pr_Game2_OW).
 qed.
 
-<<<<<<< HEAD
 end section.
-=======
-(* A family `f` of trapdoor permutations over `rand`,                   *)
-(*        indexed by `pkey`, with inverse family `fi` indexed by `skey` *)
-op f : pkey -> rand -> rand.
-op fi: skey -> rand -> rand.
-axiom fK pk sk x: (pk,sk) \in dkeys => fi sk (f pk x) = x.
-
-(* Random Oracle                                                        *)
-clone import ROM as H with
-  type in_t    <- rand,
-  type out_t   <- ptxt,
-  type d_in_t  <- unit,
-  type d_out_t <- bool,
-  op   dout _  <- dptxt.
-import Lazy.
-
-(* A Definition for OWTP Security                                       *)
-module type Inverter = {
-  proc invert(pk:pkey, x:rand): rand
-}.
-
-module Exp_OW (I : Inverter) = {
-  proc main(): bool = {
-    var pk, sk, x, x';
-
-    (pk,sk) <$ dkeys;
-    x       <$ drand;
-    x'      <@ I.invert(pk,f pk x);
-    return (x = x');
-  }
-}.
-
-(* A Definition for CPA Security                                        *)
-module type Scheme (RO : Oracle) = {
-  proc keygen(): (pkey * skey)
-  proc enc(pk:pkey, m:ptxt): ctxt
-}.
-
-module type Adv (ARO : POracle)  = {
-  proc a1(p:pkey): (ptxt * ptxt)
-  proc a2(c:ctxt): bool
-}.
-
-module CPA (O : Oracle) (S:Scheme) (A:Adv) = {
-  proc main(): bool = {
-    var pk, sk, m0, m1, c, b, b';
-
-               O.init();
-    (pk,sk) <@ S(O).keygen();
-    (m0,m1) <@ A(O).a1(pk);
-    b       <$ {0,1};
-    c       <@ S(O).enc(pk,b?m0:m1);
-    b'      <@ A(O).a2(c);
-    return b' = b;
-  }
-}.
-
-(* And a definition for the concrete Bellare-Rogaway Scheme             *)
-module (BR : Scheme) (H : Oracle) = {
-  proc keygen():(pkey * skey) = {
-    var pk, sk;
-
-    (pk,sk) <$ dkeys;
-    return (pk,sk);
-  }
-
-  proc enc(pk:pkey, m:ptxt): ctxt = {
-    var h, r;
-
-    r <$ drand;
-    h <@ H.o(r);
-    return ((f pk r) || m +^ h);
-  }
-
-  proc dec(sk:skey, c:ctxt): ptxt = {
-    var r, p, h;
->>>>>>> origin/1.0-preview
 
 type adv_cost = {
   cchoose : int; (* cost *)
@@ -637,57 +397,57 @@ module Ifind(A:Adv) = {
   proc invert(pk:pkey,y:rand): rand = {
     var m0, m1, h, b, r, x;
 
-               Hash.init();
-    (m0,m1) <@ A(Hash).choose(pk);
+               Log(LRO).init();
+    (m0,m1) <@ A(Log(LRO)).choose(pk);
     h       <$ dptxt;
-    b       <@ A(Hash).guess(y,h);
+    b       <@ A(Log(LRO)).guess(y,h);
     x <- witness; 
-    while (Hash.qs <> []){
-      r <- head witness Hash.qs; 
+    while (Log.qs <> []){
+      r <- head witness Log.qs; 
       if (f pk r = y) {
-        x <- r; Hash.qs <- [];
+        x <- r; Log.qs <- [];
       } else {
-        Hash.qs <- drop 1 Hash.qs;
+        Log.qs <- drop 1 Log.qs;
       }
     }
     return x;
   }
 }.
 
-<<<<<<< HEAD
+
 lemma ex_Reduction (cA:adv_cost) (A<:Adv [choose : `{N cA.`cchoose, #ARO.o : cA.`ochoose},
-                                          guess  : `{N cA.`cguess,  #ARO.o : cA.`oguess}] {-Hash}) &m:
+                                          guess  : `{N cA.`cguess,  #ARO.o : cA.`oguess}] {-Log, -LRO}) &m:
   (0 <= cA.`cchoose /\ 0 <= cA.`ochoose /\ 0 <= cA.`cguess /\ 0 <= cA.`oguess) =>
-  (forall (O <: ARO{-A}), islossless O.o => islossless A(O).guess) =>
+  (forall (O <: POracle{-A}), islossless O.o => islossless A(O).guess) =>
   let qH = cA.`ochoose + cA.`oguess in
   let cB = 
     4 + (4 + cf + ceqrand) * (cA.`ochoose + cA.`oguess) + cdptxt + 
     (3 + cdptxt + cget qH + cset qH + cin qH) * (cA.`ochoose + cA.`oguess) +
     cA.`cguess + cA.`cchoose in
   exists (B <: Inverter [invert : `{N cB} ]),
-    Pr[CPA(BR93(Hash), A(Hash)).main() @ &m : res] - 1%r/2%r <= Pr[OW(B).main() @ &m: res].  
+    Pr[CPA(BR93(LRO), A(LRO)).main() @ &m : res] - 1%r/2%r <= Pr[OW(B).main() @ &m: res].  
 proof.
   move=> cA_pos A_choose_ll qH.
   exists (Ifind(A)); split.  
   (* Proof of the complexity *)
   + proc.
-    seq 5 : (size Hash.qs <= cA.`ochoose + cA.`oguess) time [N((4 + cf + ceqrand) * (cA.`ochoose + cA.`oguess) + 2)] => //.
+    seq 5 : (size Log.qs <= cA.`ochoose + cA.`oguess) time [N((4 + cf + ceqrand) * (cA.`ochoose + cA.`oguess) + 2)] => //.
     + wp.
-      call (_: size Hash.qs- cA.`ochoose <= k /\ bounded RO.m (size Hash.qs);
+      call (_: size Log.qs- cA.`ochoose <= k /\ bounded LRO.m (size Log.qs);
            time
-           [(Hash.o k : [N(3 + cdptxt + cget qH + cset qH + cin qH)])]).
+           [(Log(LRO).o k : [N(3 + cdptxt + cget qH + cset qH + cin qH)])]).
       + move=> zo hzo; proc; inline *.
-        wp := (bounded RO.m qH).
+        wp := (bounded LRO.m qH).
         rnd; auto => &hr />; rewrite dptxt_ll /=; smt (cset_pos bounded_set).
-      rnd; call (_: size Hash.qs = k /\ bounded RO.m (size Hash.qs);
-           time [(Hash.o k : [N(3 + cdptxt + cget qH + cset qH + cin qH)])]).
+      rnd; call (_: size Log.qs = k /\ bounded LRO.m (size Log.qs);
+           time [(Log(LRO).o k : [N(3 + cdptxt + cget qH + cset qH + cin qH)])]).
       + move=> zo hzo; proc; inline *.
-        wp := (bounded RO.m qH).
+        wp := (bounded LRO.m qH).
         by rnd;auto => &hr />; rewrite dptxt_ll /=; smt(cset_pos bounded_set).
       inline *; auto => />; split => *.
       + smt (bounded_empty dptxt_ll size_ge0 size_eq0).
       rewrite !bigi_constz /= /#.
-    while (true) (size Hash.qs) (cA.`ochoose + cA.`oguess) time [fun _ => N(2 + cf + ceqrand)].
+    while (true) (size Log.qs) (cA.`ochoose + cA.`oguess) time [fun _ => N(2 + cf + ceqrand)].
     + move => z /=; auto => &hr H /=; smt (size_ge0).
     + move => &hr; smt (size_ge0 size_eq0). 
     + done.
@@ -697,17 +457,17 @@ proof.
   have -> //: Pr[OW(I(A)).main() @ &m : res] = Pr[OW(Ifind(A)).main() @ &m : res].
   + byequiv => //; proc; inline *; wp.
   while{2}  
-   (if Hash.qs{2} = [] then 
-       x0{2} = nth witness Hash.qs{1} (find (fun r => f pk0{2} r = y{2}) Hash.qs{1})
+   (if Log.qs{2} = [] then 
+       x0{2} = nth witness Log.qs{1} (find (fun r => f pk0{2} r = y{2}) Log.qs{1})
     else 
-     exists i, x0{2} = witness /\ 0 <= i < size Hash.qs{1} /\ Hash.qs{2} = drop i Hash.qs{1} /\ 
-               !has (fun r => f pk0{2} r = y{2}) (take i Hash.qs{1}))
-   (size Hash.qs{2}).  
+     exists i, x0{2} = witness /\ 0 <= i < size Log.qs{1} /\ Log.qs{2} = drop i Log.qs{1} /\ 
+               !has (fun r => f pk0{2} r = y{2}) (take i Log.qs{1}))
+   (size Log.qs{2}).  
   + move=> &1 z; auto => &2 />.
-    case: (Hash.qs{2}) => //= hd qs0 [i />] h0i hi hdr hhas.
-    have heq : Hash.qs{1} = take i Hash.qs{1} ++ hd :: qs0.
+    case: (Log.qs{2}) => //= hd qs0 [i />] h0i hi hdr hhas.
+    have heq : Log.qs{1} = take i Log.qs{1} ++ hd :: qs0.
     + by rewrite hdr cat_take_drop.
-    rewrite heq; move: hhas; (pose tk := take i Hash.qs{1}) => hhas.
+    rewrite heq; move: hhas; (pose tk := take i Log.qs{1}) => hhas.
     have heq1 : 
      nth witness (tk ++ hd :: qs0) (find (fun (p0 : rand) => f pk0{2} p0 = y{2}) (tk ++ hd :: qs0)) =
      nth witness (hd :: qs0) (find (fun (p0 : rand) => f pk0{2} p0 = y{2}) (hd :: qs0)).
@@ -724,77 +484,10 @@ proof.
     rewrite drop_size_cat // take_size_cat // size_rcons -cats1 has_cat /=.
     smt (size_ge0).
   wp.
-  conseq (: ={Hash.qs, pk0, x, y}).
+  conseq (: ={Log.qs, pk0, x, y}).
   + move=> /> *; split; last by smt (size_eq0 size_ge0).
     by move=> *; exists 0; rewrite drop0 take0 /=; smt (size_eq0 size_ge0).
   by sim.
-=======
-(* We will need to turn a concrete CPA adversary into an abstract one.  *)
-(*      We do not need to do it for the inverter as the types coincide. *)
-module A_CPA (A : Adv) (H : POracle) = {
-  proc a1 = A(H).a1
-
-  proc a2(c:rand * ptxt): bool = {
-    var b;
-
-    b <@ A(H).a2(c.`1 || c.`2);
-    return b;
-  }
-}.
-
-section.
-declare module A : Adv { LRO, I }.
-
-axiom A_a1_ll (O <: POracle {A}): islossless O.o => islossless A(O).a1.
-axiom A_a2_ll (O <: POracle {A}): islossless O.o => islossless A(O).a2.
-
-local clone import BR93 as Instance with
-  type pkey  <- pkey,
-  type skey  <- skey,
-  op   dkeys <- dkeys,
-  op   f     <- f,
-  op   fi    <- fi,
-  type ptxt  <- ptxt,
-  op   (+^)  <- Plaintext.(+^),
-  op   dptxt <- dptxt,
-  type rand  <- rand,
-  op   drand <- drand
-proof addA, addC, addKp, dptxt_llfuuni, drand_lluni, dkeys_llfuni, fK.
-realize addA          by move=> p1 p2 p3; algebra.
-realize addC          by move=> p1 p2; algebra.
-realize addKp         by move=> p1 p2; algebra.
-realize dptxt_llfuuni by smt(@Plaintext.DWord).
-realize drand_lluni   by smt(@Randomness.DWord).
-realize dkeys_llfuni  by exact/dkeys_llfuni.
-realize fK            by exact/fK.
-
-lemma Reduction &m:
-     Pr[CPA(LRO, BR, A).main() @ &m : res] - 1%r / 2%r
-  <= Pr[Exp_OW(Self.I(A, LRO)).main() @ &m : res].
-proof.
-have <-:   Pr[BR93_CPA(A_CPA(A)).main() @ &m: res]
-         = Pr[CPA(LRO,BR,A).main() @ &m: res].
-+ byequiv=> //=; proc.
-  inline A_CPA(A,Log(H.Lazy.LRO)).a2.
-  wp; call (: H.Lazy.LRO.m{1} = LRO.m{2}).
-  + by proc; inline *; auto.
-  inline BR93(H.Lazy.LRO).enc BR(LRO).enc H.Lazy.LRO.o LRO.o; auto.
-  call (: H.Lazy.LRO.m{1} = LRO.m{2}).
-  + by proc; inline *; auto.
-  inline *; auto=> /> [pk sk] _ [m0 m1] c b _ r _ h _ /=.
-  by rewrite addC /= addC.
-have <-:   Pr[OW_rand.OW(I(A_CPA(A))).main() @ &m: res]
-         = Pr[Exp_OW(Self.I(A,LRO)).main() @ &m: res].
-+ byequiv=> //=; proc.
-  inline *; auto; call (: H.Lazy.LRO.m{1} = LRO.m{2} /\ ={qs}(Log,Self.I)).
-  + by sim.
-  auto; call (: H.Lazy.LRO.m{1} = LRO.m{2} /\ ={qs}(Log,Self.I)).
-  + by sim.
-  by auto.
-apply/(Reduction (A_CPA(A)) _ _ &m).
-+ by move=> O O_o_ll; exact/(A_a1_ll O O_o_ll).
-by move=> O O_o_ll; proc; call (A_a2_ll O O_o_ll).
->>>>>>> origin/1.0-preview
 qed.
 
 end BR93.
